libcrux-ml-kem/proofs/fstar/extraction/Libcrux_ml_kem.Vector.Neon.Vector_type.fsti
@@ -26,6 +26,12 @@ val from_i16_array (array: t_Slice i16)
           let result:t_SIMD128Vector = result in
           repr result == array)
 
+[@@ FStar.Tactics.Typeclasses.tcinstance]
+val impl:Core.Clone.t_Clone t_SIMD128Vector
+
+[@@ FStar.Tactics.Typeclasses.tcinstance]
+val impl_1:Core.Marker.t_Copy t_SIMD128Vector
+
 val to_i16_array (v: t_SIMD128Vector)
     : Prims.Pure (t_Array i16 (sz 16))
       Prims.l_True
